a minimal interface and implementation for vcache

experiments/Veritas.VCache.fsti
@@ -1,173 +1,117 @@
 module Veritas.VCache
 
-module B = LowStar.Buffer
-module HS = FStar.HyperStack
-
+open FStar.HyperStack
 open FStar.HyperStack.ST
 
-/// Based on veritas/verifier/vcache.h
-///
-/// The vcache is a vector of entries (i.e. a dynamically-sized array of size
-/// ``CacheSize``, called ``_entries``), where each entry holds a slot. A slot
-/// is an array of 20 64-bit integers; when cast to raw bytes, this is enough
-/// space to hold either a MerkleLeafVCell or a MerkleInternalVCell. In C++,
-/// clients of the VCache call its API to obtain a pointer to a raw slot
-/// (pointer to bytes, via std::array.data), then proceed to call a placement
-/// constructor to allocate an object at that location.
-///
-/// In Low*, we go for something much simpler: we introduce a data type that is
-/// either a MerkleLeaf or a MerkleInternal. We know that KreMLin will compile
-/// this to a tagged union, whose size will be the greater of the two, meaning
-/// we implement the cache simply as an array of ``slot``.
-///
-/// This module, like the rest of the verified Veritas development, is agile
-/// over the verifier traits, a set of compile-time parameters used to
-/// specialize the code for e.g. a given cell implementation or hash algorithm.
-/// See Veritas.VerifierTraits.fsti.
+module U8 = FStar.UInt8
+module U16 = FStar.UInt16
+module U32 = FStar.UInt32
+module U64 = FStar.UInt64
+module U128 = FStar.UInt128
 
-/// Type definitions
-/// ----------------
+module HS = FStar.HyperStack
 
-/// From vcell.h
-/// class Addr: an address of a memory
-///
-/// Note: this is a value which greatly simplifies things in Low*.
-type addr = {
-  a0:UInt64.t;
-  a1:UInt64.t;
-  a2:UInt64.t;
-  a3:UInt64.t
-}
+module B = LowStar.Buffer
 
-/// From merkle.h
-/// Merkle address identifies a location in the sparse merkle tree
-type merkle_addr = {
-  path: addr;
-  depth: UInt16.t
-}
+type u8  = U8.t
+type u16 = U16.t
+type u32 = U32.t
+type u64 = U64.t
+type u128 = U128.t
 
-/// From merkle_vcell.h
-noeq
-type merkle_leaf = {
-  addr: merkle_addr;   //32 bytes
-  data_vcell: B.pointer VCell.t
-}
+type slot_id = n:u16{U16.v n < UInt.max_int U16.n}
 
-// 32 bytes
-let hash_value = UInt128.t & UInt128.t
+type u256 = u64 & u64 & u64 & u64
 
-/// From merkle_vcell.h
-///
-/// 32; 32; 64; 4; 4 = 136 <= sizeof uint64 * 20
-type merkle_internal =
-{
-   left: hash_value;    // Typically, say, 32 bytes as a pair of UInt128s
-   right: hash_value;
-   dpath: addr & addr; // Not yet sure exactly what these additional fields represent
-   depth: UInt32.t;
-   ddepth: UInt16.t & UInt16.t
-}
+type key = u256 & u8  //size of a merkle key, excluding leading zeroes
 
-/// CachePolicy, from veritas/common/common.h
-type cache_policy =
-  | Merkle
-  | Blum
-  | BlumHash
+val data_t : eqtype //Pick a concrete data value?
 
-/// A slot in the cache stores either a leaf or an internal node
-noeq
-type slot =
-  | MerkleLeaf  of merkle_leaf
-  | MerkleInternal of merkle_internal
+let data_value = option data_t
 
+(* size of a hash value *)
+let hash_size : nat = 256
 
-/// An entry is a slot paired with the metadata for use by the cache
-noeq
-type entry = {
-  slot: slot; // this is the field that is an std::array<uint64, 20> in C++
-  cp: cache_policy;
-  occupied: bool;
-  touched: bool;
-}
+(* hash value *)
+type hash_value = u128 & u128
 
-let lbuffer a l =
-  b:B.buffer a { B.length b == l }
+(* information about a desc stored in a merkle node *)
+type descendent_hash =
+  | Empty: descendent_hash
+  | Desc: k:key -> //Q: do we really need to store this here? I guess because its sparse we can't compute the key of the descendent?
+          h:hash_value ->
+          evicted_to_blum:bool -> //Q: What does this represent?
+          in_store:bool -> //The descendent with key k is in the VStore
+          descendent_hash
 
-/// The main type provided by vcache encapsulates a fixed array of
-/// cache entries.
-///
-/// Note that the run-time representation does not depend on t (otherwise, a
-/// trick like https://github.com/FStarLang/kremlin/issues/183 would be needed).
-///
-/// TODO: hide this behind the abstraction once it's ready.
-noeq
-type t (tr: VerifierTraits.t) = {
-  entries: lbuffer entry (UInt16.v tr.VerifierTraits.cache_size)
-}
+type value =
+  | MVal : l:descendent_hash -> r:descendent_hash -> value
+  | DVal : data_value -> value
 
-/// Stateful API
-/// ------------
-///
-/// In order to make sure you're not forgetting anything, it's always a good
-/// idea to refer to hacl-star/code/streaming/Hacl.Streaming.Interface and make
-/// sure you're implementing at least the stateful type class, which is the bare
-/// minimum for your clients to be able to do something with your code.
+type record = key & value
 
-/// We have some abstract invariants on caches, e.g., liveness properties etc.
-/// This also includes freeable, which we'll need to implement the free function.
-val invariant (#tr: VerifierTraits.t) (h: HS.mem) (cache: t tr): Type0
+type add_method =
+  | MAdd: add_method  (* AddM *)
+  | BAdd: add_method  (* AddB *)
 
-/// We aim for a static footprint. Note that this is just about the array of
-/// entries, knowing that vcells are values means that we don't have to be more
-/// complicated than that.
-val footprint (#tr: VerifierTraits.t) (cache: t tr): GTot B.loc
+val most_significant_bit (k:key) : bool
 
-val invariant_loc_in_footprint: #tr:VerifierTraits.t -> h:HS.mem -> cache:t tr -> Lemma
-    (requires (invariant h cache))
-    (ensures (B.loc_in (footprint cache) h))
-    [ SMTPat (invariant h cache) ]
+let is_data_key (k:key) : bool = most_significant_bit k
 
-/// For spec purposes, a cache is a sequence of entries
-val entries (#tr: VerifierTraits.t) (h: HS.mem) (cache: t tr):
-  GTot (Seq.lseq entry (UInt16.v (tr.VerifierTraits.cache_size)))
+let is_value_of (k:key) (v:value)
+  : bool
+  = if is_data_key k then DVal? v else MVal? v
 
-val frame_invariant: #tr:VerifierTraits.t -> l:B.loc -> cache:t tr -> h0:HS.mem -> h1:HS.mem -> Lemma
-    (requires (
-      invariant h0 cache /\
-      B.loc_disjoint l (footprint cache) /\
-      B.modifies l h0 h1))
-    (ensures (
-      invariant h1 cache /\
-      entries h0 cache == entries h1 cache /\
-      footprint cache == footprint cache))
-    [ SMTPat (invariant h1 cache); SMTPat (B.modifies l h0 h1) ]
+val vstore : Type0
 
-/// Cache entries are indexed by u16 values
-let vcache_idx = UInt16.t
+val invariant (st:vstore) (h:HS.mem) : Type0
 
-/// The C++ API allows looking up cache entries and returns them by reference.
-/// These references are then read and mutated by client code in vmem_vops.h etc.
-///
-/// We go for something simpler and assume clients of this module will keep
-/// track of an index, rather than manipulate raw values (this would greatly
-/// complicate the framing lemmas).
+val footprint (st:vstore) : GTot B.loc
 
-/// Note that this returns a value via a dereference.
-val get_entry (#tr: VerifierTraits.t) (cache: t tr) (idx: vcache_idx { idx `FStar.UInt16.lt` tr.VerifierTraits.cache_size }):
-  Stack entry
-    (requires fun h0 ->
-      invariant h0 cache)
-    (requires fun h0 e h1 ->
-      e == Seq.index (entries h0 cache) (UInt16.v idx) /\
-      h0 == h1)
+val as_seq (st:vstore) (h:HS.mem)
+  : GTot (Seq.lseq (option record) (UInt.max_int U16.n))
 
-val set_entry (#tr: VerifierTraits.t) (cache: t tr)
-  (idx: vcache_idx { idx `FStar.UInt16.lt` tr.VerifierTraits.cache_size })
-  (entry: entry):
-  Stack unit
-    (requires fun h0 ->
-      invariant h0 cache)
-    (requires fun h0 _ h1 ->
-      invariant h1 cache /\
-      B.modifies (footprint cache) h0 h1 /\
-      entries h1 cache == Seq.upd (entries h0 cache) (UInt16.v idx) entry)
+val vcache_create (_:unit)
+  : ST vstore
+      (requires fun h -> True)
+      (ensures fun h0 st h1 ->
+        B.(modifies loc_none h0 h1) /\
+        invariant st h1 /\
+        B.fresh_loc (footprint st) h0 h1 /\
+        as_seq st h1 == Seq.create (UInt.max_int U16.n) None)
+
+val vcache_get_record (st:vstore) (s:slot_id)
+  : Stack (option record)
+      (requires fun h -> invariant st h)
+      (ensures fun h0 r h1 ->
+        h0 == h1 /\
+        r == Seq.index (as_seq st h1) (U16.v s))
+
+val vcache_update_record (st:vstore) (s:slot_id) (r:record)
+  : Stack unit
+      (requires fun h -> invariant st h)
+      (ensures fun h0 _ h1 ->
+        B.(modifies (footprint st) h0 h1) /\
+        invariant st h1 /\
+        as_seq st h1 == Seq.upd (as_seq st h0) (U16.v s) (Some r))
+
+val vcache_add_record  //AR: Difference from vcache_update_record?
+  (st:vstore)
+  (s:slot_id)
+  (k:key)
+  (v:value{is_value_of k v})
+  (a:add_method)
+  : Stack unit
+      (requires fun h -> invariant st h)
+      (ensures fun h0 _ h1 ->
+        B.(modifies (footprint st) h0 h1) /\
+        invariant st h1 /\
+        as_seq st h1 == Seq.upd (as_seq st h0) (U16.v s) (Some (k, v)))
+
+val vcache_evict_record (st:vstore) (s:slot_id) (k:key)  //AR: Do we need k here?
+  : Stack unit
+      (requires fun h -> invariant st h)
+      (ensures fun h0 _ h1 ->
+        B.(modifies (footprint st) h0 h1) /\
+        invariant st h1 /\
+        as_seq st h1 == Seq.upd (as_seq st h0) (U16.v s) None)
